Handling of AsmStmt in c-parser, more tests.
The C-parser contains a full parser for __asm__ syntax but
up until now hasn't done anything with it. Instead we export
some semantics. It's unspecified exactly what these semantics
are but they are parametrised with the __asm__ semantics that
went in to them, so the translation validation has something
to reason about.

Tweak modifies proofs as a result, and add some more test files.

tools/asmrefine/testfiles/global_array_swap.c
@@ -1,0 +1,88 @@
+/*
+ * Copyright 2016, Data61
+ *
+ * This software may be distributed and modified according to the terms of
+ * the BSD 2-Clause license. Note that NO WARRANTY is provided.
+ * See "LICENSE_BSD2.txt" for details.
+ *
+ * @TAG(NICTA_BSD)
+ */
+
+typedef unsigned int uint32_t;
+typedef unsigned char uint8_t;
+typedef unsigned long word_t;
+
+struct blob {
+    uint32_t words[2];
+};
+typedef struct blob blob_t;
+
+enum _bool {
+    false = 0,
+    true = 1
+};
+
+typedef struct range_blob {
+    word_t start;
+    word_t end;
+} range_blob_t;
+
+typedef struct struct_blob {
+    word_t index;
+    uint8_t data1;
+    uint8_t data2;
+    uint8_t data3;
+    uint8_t data4;
+} struct_blob_t;
+
+typedef struct {
+    word_t id;
+    word_t index;
+
+    range_blob_t index_range;
+    range_blob_t free_index_range;
+
+    void* ptr_to_stuff; /* pointer to initial thread's IPC buffer */
+    range_blob_t range_in_stuff;
+    range_blob_t next_range_in_stuff;
+
+    struct_blob_t list_of_data[192];
+
+    range_blob_t used_part_of_list;
+} big_struct_t;
+
+typedef struct toplevel_struct {
+    range_blob_t a_range;
+    int config_data1;
+    int config_data2;
+
+    big_struct_t *things;
+} toplevel_struct_t;
+
+int a_modified_global;
+int another_global;
+extern toplevel_struct_t toplevel;
+
+void
+modify_toplevel (int x)
+{
+  toplevel.config_data1 = x;  
+}
+
+void
+add_a_thing (int thing_num, int data_num)
+{
+    if (data_num < 192) {
+      toplevel.things[thing_num].list_of_data[data_num].index = 1;
+    }
+    else {
+      toplevel.things[thing_num].range_in_stuff.end = -1;
+    }
+}
+
+void
+update_a_global (int x) {
+  a_modified_global = x;
+}
+
+
