proof/asmrefine/TestGraphRefine.thy
@@ -53,12 +53,48 @@ where
             (hrs_mem (t_hrs_' (globals s)))
         \<and> htd_safe domain (hrs_htd (t_hrs_' (globals s)))}"
 
-ML {* ProveSimplToGraphGoals.test_all_graph_refine_proofs_after
-    funs (csenv ()) @{context} (SOME "Kernel_C.lookupPTSlot")  *}
+abbreviation(input) "ghost_assns_from_globals
+    \<equiv> (snd o snd o ghost'state_' :: globals \<Rightarrow> _)"
 
-ML {* val nm = "Kernel_C.lookupPTSlot" *}
+lemma snd_snd_gs_new_frames_new_cnodes[simp]:
+  "snd (snd (gs_new_frames sz ptr bits gs)) = snd (snd gs)"
+  "snd (snd (gs_new_cnodes sz' ptr bits gs)) = snd (snd gs)"
+  "snd (snd (gs_clear_region ptr sz' gs)) = snd (snd gs)"
+  "snd (snd ((if P then f else g) gs)) = (if P then snd (snd (f gs)) else snd (snd (g gs)))"
+  by (simp_all add: gs_new_frames_def gs_new_cnodes_def gs_clear_region_def)
+
+ML {* ProveSimplToGraphGoals.test_all_graph_refine_proofs_after
+    funs (csenv ()) @{context} NONE  *}
+
+ML {* val nm = "Kernel_C.dmb" *}
 
 local_setup {* define_graph_fun_short funs nm *}
+
+schematic_goal "\<And>Q. simpl_to_graph \<Gamma> GG ''Kernel_C.dmb'' (NextNode 2)
+                                           (add_cont
+                                             (Spec (asm_spec (\<lambda>s. t_hrs_' (globals s))
+                                                     (\<lambda>u. globals_update (t_hrs_'_update u))
+                                                     (\<lambda>s. phantom_machine_state_' (globals s))
+                                                     (\<lambda>u. globals_update (phantom_machine_state_'_update u))
+                                                     True ''dmb'' (\<lambda>x s. s) (\<lambda>s. [])))
+                                             [Inr SKIP])
+                                           0 [Q] UNIV simpl_invariant ?eqs
+                                           (\<lambda>s s'. var_acc ''Mem'' s =
+                                                   VarMem (hrs_mem (t_hrs_' (gswap (globals s')))) \<and>
+                                                   var_acc ''HTD'' s =
+                                                   VarHTD (hrs_htd (t_hrs_' (globals s'))) \<and>
+                                                   var_acc ''PMS'' s =
+                                                   VarMS (encode_machine_state
+    (phantom_machine_state_' (globals s'))) \<and>
+                                                   var_acc ''GhostAssertions'' s =
+                                                   VarWordArray64_32
+                                                    ((snd \<circ> snd \<circ> ghost'state_') (globals s')) \<and>
+                                                   [] = []) "
+  apply (rule simpl_to_graph_call_asm_fun[OF refl])
+  apply (tactic {* SimplToGraphProof.inst_graph_tac @{context} 1 *})
+  apply (tactic {* SimplToGraphProof.apply_asm_refines_ex_tac funs @{context} 1 *})
+  using asm_semantics_respects [[show_types]]
+  apply (rule asm_semantics_respects)
 
 ML {*
 val hints = SimplToGraphProof.mk_hints funs @{context} nm
@@ -82,16 +118,23 @@ val full_goal_tac = ProveSimplToGraphGoals.graph_refine_proof_full_goal_tac
     (csenv ())
 *}
 
-schematic_lemma "PROP ?P"
-  apply (tactic {* rtac init_thm 1 *})
+schematic_goal "PROP ?P"
+  apply (tactic {* resolve_tac @{context} [init_thm] 1 *})
   
   apply (tactic {* ALLGOALS (fn i => fn t => 
     let val res = try ((full_goal_tac @{context} THEN_ALL_NEW K no_tac) i #> Seq.hd) t
     in case res of NONE => Seq.single t | SOME r => Seq.single r
     end) *})
 
+
+
+
   apply (tactic {* ALLGOALS (nth (tacs @{context}) 0) *})
   apply (tactic {* ALLGOALS (nth (tacs @{context}) 1) *})
+
+  apply (simp_all only: globals_swap_twice[OF globals_list_distinct])
+
+
 
   apply (tactic {* ALLGOALS (nth (tacs @{context}) 2) *})
 
