tools/asmrefine/testfiles/global_array_swap.thy
@@ -1,0 +1,38 @@
+(*
+ * Copyright 2016, Data61
+ *
+ * This software may be distributed and modified according to the terms of
+ * the BSD 2-Clause license. Note that NO WARRANTY is provided.
+ * See "LICENSE_BSD2.txt" for details.
+ *
+ * @TAG(NICTA_BSD)
+ *)
+
+theory global_array_swap
+
+imports
+  "../../c-parser/CTranslation" "../GlobalsSwap"
+begin
+
+declare [[populate_globals=true]]
+
+typedecl machine_state
+typedecl cghost_state
+
+install_C_file "global_array_swap.c"
+  [machinety=machine_state, ghostty=cghost_state]
+
+setup {* DefineGlobalsList.define_globals_list_i
+  "global_array_swap.c" @{typ globals} *}
+
+locale target
+  = global_array_swap_global_addresses
+begin
+
+abbreviation
+ "globals_list \<equiv> global_array_swap_global_addresses.global_data_list"
+lemmas global_data_defs = global_array_swap_global_addresses.global_data_defs
+
+end
+
+end
